LogicalRefinement/Untyped/Wk.lean
@@ -9,6 +9,7 @@ import LogicalRefinement.Untyped.Basic
   | let_bin k e => let_bin k (wk (RawWk.liftn 2 ρ) e)
   | bin k l r => bin k (wk ρ l) (wk ρ r)
   | abs k A t => abs k (wk ρ A) (wk (RawWk.lift ρ) t)
+  | tri k A l r => tri k (wk ρ A) (wk ρ l) (wk ρ r)
   | cases k K d l r => cases k (wk (RawWk.lift ρ) K) (wk ρ d) (wk ρ l) (wk ρ r)
 
 @[simp] def RawUntyped.wk1 (u: RawUntyped) := wk RawWk.wk1 u
@@ -33,6 +34,7 @@ import LogicalRefinement.Untyped.Basic
     intros ρ σ H;
     simp only [wk];
     simp only [IHA H, IHs (RawWk.lift_equiv H)]
+  | tri k A l r IA Il Ir => intros ρ σ H; simp [IA H, Il H, Ir H]
   | cases k K d l r IK Id Il Ir => 
     intros ρ σ H; 
     simp only [wk];
@@ -53,6 +55,7 @@ import LogicalRefinement.Untyped.Basic
     simp only [wk]
     rw [RawUntyped.wk_coherent RawWk.lift_id_equiv]
     rw [IHA, IHs]
+  | tri k A l r IA Il Ir => simp [IA, Il, Ir]
   | cases k K d l r IK Id Il Ir => 
     simp only [wk]
     rw [RawUntyped.wk_coherent RawWk.lift_id_equiv]
@@ -89,6 +92,16 @@ def RawUntyped.wk_bounds {u: RawUntyped}: {n m: Nat} -> {ρ: RawWk} ->
       case abs.right => 
         let Hm' := @wk_maps_liftn 1 n m ρ Hm
         apply IHs Hm' Hs
+    | tri k A l r IHA IHl IHr =>
+      simp only [fv, Nat.max_r_le_split]
+      intros n m ρ Hm
+      intro ⟨HA, Hl, Hr⟩
+      apply And.intro;
+      case left => apply IHA Hm HA
+      case right =>
+        apply And.intro;
+        case left => apply IHl Hm Hl
+        case right => apply IHr Hm Hr
     | cases k K d l r IK IHd IHl IHr => 
       simp only [fv, Nat.max_r_le_split, Nat.le_sub_is_le_add]
       intros n m ρ Hm
@@ -118,6 +131,7 @@ def RawUntyped.fv_wk1: fv (wk1 u) ≤ fv u + 1 := by {
   | let_bin k t I => simp [I]
   | bin k l r Il Ir => simp [Il, Ir]
   | abs k A t IA It => simp [IA, It] 
+  | tri k A l r IA Il Ir => simp [IA, Il, Ir]
   | cases k K d l r IK Id Il Ir => simp [IK, Id, Il, Ir]
 }
 
